Isolate all non-linear arithmetic reasoning

src/Dafny/util/pow.dfy
@@ -2,28 +2,63 @@
 Uninteresting definition of pow (exponentiation)
 */
 
+include "../nonlin/arith.dfy"
+
 module Pow {
 
-function method pow(x:nat, k:nat): (p:nat) decreases k
-ensures 1 <= x ==> 1 <= p
-{
-    if k == 0 then 1 else x * pow(x,k-1)
-}
+    import opened Arith
 
-lemma {:induction k1} pow_plus(x: nat, k1: nat, k2: nat)
-ensures pow(x, k1) * pow(x, k2) == pow(x, k1+k2)
-{}
+    function method pow(x:nat, k:nat): (p:nat)
+        decreases k
+    {
+        if k == 0 then 1 else (
+            mul_positive(x, pow(x,k-1));
+            x * pow(x,k-1)
+        )
+    }
 
-lemma {:induction k} pow_pos(x: nat, k: nat)
-requires 0 < x
-ensures 0 < pow(x, k)
-{}
+    lemma {:induction k1} pow_plus(x: nat, k1: nat, k2: nat)
+        decreases k1
+        ensures pow(x, k1) * pow(x, k2) == pow(x, k1+k2)
+    {
+        if k1 == 0 {
+            calc {
+                pow(x, k1) * pow(x, k2);
+                1 * pow(x, k2);
+                pow(x, k2);
+                pow(x, k1+k2);
+            }
+        } else {
+            calc {
+                pow(x, k1) * pow(x, k2);
+                x * pow(x,k1-1) * pow(x, k2);
+                { pow_plus(x, k1-1, k2); }
+                { mul_assoc(x, pow(x,k1-1), pow(x, k2)); }
+                x * pow(x, (k1-1) + k2);
+                pow(x, k1+k2);
+            }
+        }
+    }
 
-lemma {:induction k1} pow_increasing(x: nat, k1: nat, k2: nat)
-requires 0 < x
-ensures pow(x, k1) <= pow(x, k1+k2)
-{
-    pow_plus(x, k1, k2);
-}
+    lemma {:induction k} pow_pos(x: nat, k: nat)
+        decreases k
+        requires 0 < x
+        ensures 0 < pow(x, k)
+    {
+        if k == 0 {
+        } else {
+            pow_pos(x, k-1);
+            mul_r_increasing(pow(x, k-1), x);
+        }
+    }
+
+    lemma {:induction false} pow_increasing(x: nat, k1: nat, k2: nat)
+        requires 0 < x
+        ensures pow(x, k1) <= pow(x, k1+k2)
+    {
+        pow_plus(x, k1, k2);
+        pow_pos(x, k2);
+        mul_r_increasing(pow(x, k1), pow(x, k2));
+    }
 
 }
