src/Dafny/.dir-locals.el
@@ -1,0 +1,4 @@
+;;; Directory Local Variables
+;;; For more information see (info "(emacs) Directory Variables")
+
+((dafny-mode . ((dafny-prover-local-args . ("/z3opt:smt.arith.nl=false" "/arith:5")))))
